The mini project language

Mjollnir.v
@@ -9,14 +9,22 @@ Require Import Integers.
 (* ToDo: Add Mach to contrib (many dependencies) *)
 Definition regset := Regmap.t val.
 
+Inductive expr : Type :=
+  | intlit : val -> expr
+  | add : positive -> positive -> expr.
+
 Inductive stmt : Type :=
-  | nop : stmt.
+  | skip : stmt
+  | assign : positive -> expr -> stmt.
 
 Definition path : Type := list stmt.
 
 Definition state : Type := regset.
+
+Definition empty_state : state := Regmap.init Vundef.
+
 Definition v := ((Regmap.init (Vint (Int.repr 5))) # 1).
-Eval compute in ((Regmap.init (Vint (Int.repr 5))) # 1).
+Eval compute in v.
 
 
 Inductive correlation : Type :=
@@ -27,10 +35,53 @@ Inductive correlation_holds : correlation -> state -> state -> Prop :=
   | states_eq_holds : forall st, correlation_holds states_eq st st
   | true_c_holds    : forall st1 st2, correlation_holds true_c st1 st2.
 
-Definition step (s0:state) (stmt:stmt) : state :=
-  s0.
+Definition add_int_vals v1 v2 : val :=
+  match (v1, v2) with
+    | (Vint x, Vint y) => Vint (Int.add x y)
+    | _                => Vint (Int.zero)
+  end.
+
+Definition eval (s:state) (e:expr) : val :=
+  match e with
+    | intlit x => x
+    | add v1 v2 => add_int_vals (s#v1) (s#v2)
+  end.
+
+Definition step (s:state) (stmt:stmt) : state :=
+  match stmt with
+    | skip => s
+    | assign var e => 
+      let val := eval s e 
+        in s # var <- val
+  end.
 
 Definition step_path s0 p := fold_left step p s0.
+
+(* ToDo: Look at Zach's stuff and fix better notation *)
+
+Definition my_program :=
+  assign 1 (intlit (Vint (Int.repr 5))) ::
+  assign 2 (intlit (Vint (Int.repr 3))) ::
+  assign 3 (add 1 2)                    ::
+  nil.
+
+Definition my_program_opt :=
+  assign 1 (intlit (Vint (Int.repr 5))) ::
+  assign 2 (intlit (Vint (Int.repr 3))) ::
+  assign 3 (intlit (Vint (Int.repr 8))) ::
+  nil.
+
+Lemma my_program_opt_correct : 
+  correlation_holds states_eq
+  (step_path empty_state my_program)
+  (step_path empty_state my_program_opt).
+Proof.
+  apply states_eq_holds. (* Wow! *)
+Qed.
+
+Eval compute in (step_path empty_state my_program_opt) # 3.
+
+
 
 Definition pec_check (c c':correlation) (p1 p2:path) : bool :=
   true.
